WIP

ModalTypes/Context.lean
@@ -1,4 +1,5 @@
 import ModalTypes.Type
+import Mathlib.Tactic.Linarith
 
 /-!
   In the paper, a context is presented as an (ordered) sequence of types and locks.
@@ -11,15 +12,71 @@ abbrev Context : Type :=
 
 namespace Context
 
+/-- 
+  Add a new variable to the top-most sub-context, 
+  creating a new sub-context if none exists yet -/
 def add (t : Ty) : Context → Context
   | [] => [[t]]
   | Γ::Γs => (t::Γ)::Γs
+
+/--
+  Add a new lock to the context
+-/
+def addLock : Context → Context :=
+  fun Γ => []::Γ
 
 def get? (Γ : Context) : (Nat × Nat) → Option Ty
   | ⟨i, j⟩ => List.get? Γ i |>.bind (List.get? · j)
 
 def Var (Γ : Context) (ty : Ty) : Type :=
   { i // Γ.get? i = some ty}
+
+/-- 
+  The total number of vars in this context.
+  That is, the sum of the number of vars in each sub-context, disregarding the locks
+-/
+def vars : Context → Nat :=
+  Nat.sum ∘ List.map (List.length)
+
+open TypeScheme in
+/--
+  Given a context `Γ` and an expected type `A`, we can determine the denotation of a judgement
+    `Γ ⊢ _ : A`
+  as a formula (type)
+  Note that this denotation depends only on `Γ` and `A`, not on the structure of the proof, hence
+  it is defined here.
+-/
+def denote : Context → Ty → Ty
+  | [],           A => A
+  | (B::Bs)::Γs,  A => ⟪B → ${denote (Bs::Γs) A}⟫
+  | []::Γs,       A => ⟪ □${denote Γs A} ⟫
+
+notation (priority := high) "⟦ " Γ " ⊢ _ : " t " ⟧" => denote Γ t 
+
+
+
+
+/-
+  ## Theorems
+-/
+
+@[simp]
+theorem vars_add :
+    vars (add A Γ) = vars Γ + 1 := by
+  simp only [vars, add, Function.comp]
+  cases Γ 
+  . rfl
+  . simp only [List.map, List.length_cons, Nat.sum_cons]; linarith
+
+@[simp]
+theorem vars_cons :
+    vars (Γ :: Γs) = Γ.length + vars Γs := by
+  rfl
+
+@[simp]
+theorem vars_append :
+    vars (Γ ++ Γ') = vars Γ + vars Γ' := by
+  simp only [vars, Function.comp_apply, List.map_append, Nat.sum_append]
 
 end Context
 
