ModalTypes/Hilbert.lean
@@ -1,4 +1,5 @@
 import ModalTypes.Type
+import ModalTypes.Context
 import Mathlib.Data.Vector.Basic
 
 open TypeScheme
@@ -13,10 +14,12 @@ namespace Axioms
   This is a Hilbert-style axiomatic proof.
 -/
 inductive Proof (axioms : Axioms) : {n : Nat} → TypeScheme n → Prop
-  | axiom : (∃i, axioms.get i = ⟨n, t⟩) → Proof axioms t
+  | axiom : (∃i, axioms.get? i = some ⟨n, A⟩) → Proof axioms A
   | modusPonens {A B : TypeScheme n} : 
       Proof axioms ⟪A → B⟫ → Proof axioms A → Proof axioms B
-  | substitution (f : Fin n → TypeScheme m) : Proof axioms A → Proof axioms (A.substitute f)
+  | substitution ⦃n : Nat⦄ {A : TypeScheme n} (h : Proof axioms A)
+      (f : Fin n → TypeScheme m) (h_eq : A.substitute f = A' := by rfl) : 
+      Proof axioms A'
   /--
     Rule of necessitation: if `A` is a theorem, then so is `□A`.
     Note that this is different from having `A → □A` as an axiom!
@@ -24,13 +27,16 @@ inductive Proof (axioms : Axioms) : {n : Nat} → TypeScheme n → Prop
   | necessitation : Proof axioms A → Proof axioms ⟪ □A ⟫
 
 
+/-
+  # Axiom Sets
+-/
 
 /-- The basic axioms of propositional, intuitionistic logic 
     https://en.wikipedia.org/wiki/Intuitionistic_logic
 -/
 def propLogic : Axioms := [
   ⟨2, ⟪ %0 → %1 → %0 ⟫⟩,  -- THEN-1
-  ⟨3, ⟪ (%0 → (%1 → %2)) → (%0 → %1) → (%0 → %2) ⟫⟩, -- THEN-2
+  ⟨3, ⟪ (%0 → %1 → %2) → (%0 → %1) → (%0 → %2) ⟫⟩, -- THEN-2
   ⟨2, ⟪ %0 × %1 → %0 ⟫⟩, -- AND-1
   ⟨2, ⟪ %0 × %1 → %1 ⟫⟩, -- AND-2
   ⟨2, ⟪ %0 → %1 → %0 × %1 ⟫⟩, -- AND-3
@@ -43,5 +49,78 @@ def propLogic : Axioms := [
 def K : Axioms := propLogic ++ [
   ⟨2, ⟪ □(%0 → %1) → □%0 → □%1 ⟫⟩
 ]
+
+/-
+  # Theorems
+-/
+
+/-- Adding more axioms does not invalidate earlier theorems -/
+theorem Proof.append_axioms (h : Proof axioms A) : Proof (axioms ++ newAxioms) A := by
+  induction h
+  next h =>
+    apply Proof.axiom
+    rcases h with ⟨i, h⟩
+    use i
+    rw [List.get?_append (List.get?_eq_some.mp h).1]
+    apply h
+  next ih₁ ih₂ => apply Proof.modusPonens ih₁ ih₂
+  next f h_eq ih => apply ih.substitution f h_eq
+  next ih => apply Proof.necessitation ih
+
+theorem THEN₁ : Proof propLogic (n:=2) ⟪ %0 → %1 → %0 ⟫ :=
+  .axiom ⟨0, rfl⟩
+
+theorem THEN₂ : Proof propLogic (n:=3) ⟪ (%0 → %1 → %2) → (%0 → %1) → (%0 → %2) ⟫ :=
+  .axiom ⟨1, rfl⟩
+
+theorem OR₁ : Proof propLogic (n:=2) ⟪ %0 → %0 + %1 ⟫ :=
+  .axiom ⟨5, rfl⟩
+
+theorem THEN_id : Proof propLogic (n:=1) ⟪ %0 → %0 ⟫ :=
+  have t₁ := THEN₁.substitution (m:=1) (fun 
+      | 0 => ⟪%0⟫
+      | 1 => ⟪%0 + %0⟫
+    )
+  have t₂ := THEN₂.substitution (m:=1) (fun
+      | 0 => ⟪%0⟫
+      | 1 => ⟪%0 + %0⟫
+      | 2 => ⟪%0⟫
+    )
+  have o₁ := OR₁.substitution (m:=1) (fun _ => ⟪%0⟫)
+  .modusPonens (t₂.modusPonens t₁) o₁
+
+-- theorem THEN_a_to_b_to_c :Proof propLogic (n:=3) ⟪(%0 → %2) → %0 → %1 → %2⟫ := by
+--   -- have t : Proof _ ⟪ (%0 → %0 → %1 → %2) → (%0 → %0) → (%0 → %1 → %2) ⟫ := THEN₂.substitution (m:=3) (fun
+--   --   | 0 => ⟪ %0 ⟫
+--   --   | 1 => ⟪ %0 ⟫
+--   --   | 2 => ⟪ %1 → %2 ⟫
+--   -- ) 
+--   sorry
+
+-- theorem implication (h : Proof ax A → Proof Ax B) : Proof ax ⟪ A → B ⟫ := by
+--   sorry
+
+/-
+  # Context denotation
+-/
+
+-- open Proof in
+-- theorem denote_ofResult : Proof K ⟪A → ${⟦ Γ ⊢ _ : A ⟧}⟫ := by
+--   induction Γ
+--   next => 
+--     exact THEN_id.append_axioms.substitution (fun _ => A)
+--   next Γ Γs ih =>
+--     induction Γ <;> simp only [Context.denote]
+--     next => 
+--       -- apply Proof.necessitation ih
+--       sorry
+--     next hd tl ih₂ =>
+--       apply Proof.modusPonens _ ih₂
+--       -- apply THEN₁.append_axioms.substitution (fun
+--       --     | 0 => ⟦ tl :: Γs ⊢ _ : A ⟧
+--       --     | 1 => hd
+--       --   )
+--       sorry
+      
 
 end Axioms
