ModalTypes/Term.lean
@@ -12,12 +12,49 @@ inductive Term
   | inr : Term → Term
   | fst : Term → Term
   | snd : Term → Term
+  | case (t u₁ u₂ : Term) : Term
   /-- open a box modality -/
   | open : Term → Term
   /-- shut a box modality -/
   | shut : Term → Term
 
--- inductive Term : Context → Ty → Type
---   | var : Var Γ t → Term Γ t
---   | lam : (t : Ty) → Term (t::Γ) u → Term Γ (.fun t u)
---   | prod : 
+
+
+
+namespace Term
+
+/-- 
+  A term is closed if it has no free variables. 
+  Auxiliary definition where variables strictly less than `b` are considered bound 
+-/
+def IsClosedUpTo (b : Nat) : Term → Prop
+  | var n         => n < b
+  | lam _ t       => IsClosedUpTo (b+1) t
+  | app t u       => IsClosedUpTo b t ∧ IsClosedUpTo b u
+  | pair t u      => IsClosedUpTo b t ∧ IsClosedUpTo b u
+  | inl t         => IsClosedUpTo b t
+  | inr t         => IsClosedUpTo b t
+  | fst t         => IsClosedUpTo b t
+  | snd t         => IsClosedUpTo b t
+  | case t u₁ u₂  => IsClosedUpTo b t ∧ IsClosedUpTo (b+1) u₁ ∧ IsClosedUpTo (b+1) u₂
+  | «open» t      => IsClosedUpTo b t
+  | shut t        => IsClosedUpTo b t
+
+/-- A term is closed if it has no free variables -/
+abbrev IsClosed : Term → Prop := IsClosedUpTo 0
+
+
+
+theorem isClosedUpTo_succ {t : Term} : t.IsClosedUpTo n → t.IsClosedUpTo (n+1) := by
+  intro h
+  induction t generalizing n <;> simp_all [IsClosedUpTo]
+  . apply Nat.lt_add_right _ _ _ h
+
+theorem isClosedUpTo_add {t : Term} : t.IsClosedUpTo n → t.IsClosedUpTo (n+m) := by
+  intro h
+  induction m
+  next    => exact h
+  next ih => apply isClosedUpTo_succ ih
+
+
+end Term
