ModalTypes/WellTyped.lean
@@ -1,9 +1,10 @@
 import ModalTypes.Term
 import ModalTypes.Type
 import ModalTypes.Context
+import ModalTypes.Hilbert
 import Aesop
 
-open Ty 
+open TypeScheme -- for notation
 
 @[aesop safe constructors]
 inductive WellTyped : Context → Term → Ty → Prop
@@ -17,13 +18,15 @@ inductive WellTyped : Context → Term → Ty → Prop
   /-- Standard rule for application -/
   | app (A) : WellTyped Γ f ⟪ A → B⟫ → WellTyped Γ t A → WellTyped Γ (.app f t) B
   /-- Standard rule for products -/
-  | prod : WellTyped Γ t A → WellTyped Γ u B → WellTyped Γ (.pair t u) ⟪ A × B ⟫
+  | pair : WellTyped Γ t A → WellTyped Γ u B → WellTyped Γ (.pair t u) ⟪ A × B ⟫
   /-- Standard rule for sums -/
   | inl : WellTyped Γ t A → WellTyped Γ (.inl t) ⟪ A + B ⟫
   /-- Standard rule for sums -/
   | inr : WellTyped Γ t B → WellTyped Γ (.inr t) ⟪ A + B ⟫
   | fst : WellTyped Γ t ⟪ A × B ⟫ → WellTyped Γ (.fst t) A
   | snd : WellTyped Γ t ⟪ A × B ⟫ → WellTyped Γ (.snd t) B
+  | case : WellTyped Γ t ⟪ A + B ⟫ → WellTyped (Γ.add A) u₁ C → WellTyped (Γ.add B) u₂ C
+    → WellTyped Γ (.case t u₁ u₂) C
   /-
     TODO: in this encoding of the shut rule, `Γ'` cannot contain any more locks, but the original
       has no such restriction.
@@ -32,19 +35,211 @@ inductive WellTyped : Context → Term → Ty → Prop
       (I choose this second option for now)
   -/
   | open : WellTyped Γ t ⟪ □A ⟫ → WellTyped (Γs ++ Γ'::Γ) (.open t) A
-  | shut : WellTyped ([]::Γ) t A → WellTyped Γ (.shut t) ⟪ □A ⟫
+  | shut : WellTyped Γ.addLock t A → WellTyped Γ (.shut t) ⟪ □A ⟫
+
+
+namespace WellTyped
+
+notation Γ " ⊢ " t " : " A => WellTyped Γ t A
+notation "⊢ " t " : " A => WellTyped [] t A
 
 
 
-example : ∃ t, WellTyped [] t ⟪ □(A → B) → □A → □B ⟫ := by
+/-
+  # Completeness
+-/
+
+open Axioms (K Proof THEN₁)
+
+namespace Completeness
+
+abbrev Inhabited (A : Ty) : Prop :=
+  ∃t, ⊢ t : A 
+
+theorem THEN₁ : Inhabited ⟪ A → B → A ⟫ := ⟨
+    .lam A <| .lam B <| .var 1, 
+    .lam <| .lam <| .var rfl
+  ⟩
+
+theorem THEN₂ : Inhabited ⟪ (A → B → C) → (A → B) → (A → C) ⟫ := ⟨
+    .lam ⟪A → B → C⟫ <| .lam ⟪A → B⟫ <| .lam A <| .app 
+      (.app (.var 2) (.var 0)) 
+      (.app (.var 1) (.var 0)), 
+    by
+      apply lam <| lam <| lam _
+      apply app
+      . apply app
+        . apply var; rfl
+        . apply var; rfl
+      . apply app
+        . apply var; rfl
+        . apply var; rfl
+  ⟩
+
+theorem AND₁ : Inhabited ⟪ A × B → A ⟫ := ⟨
+  .lam ⟪A × B⟫ <| .fst <| .var 0,
+  lam <| fst <| var rfl
+⟩
+
+theorem AND₂ : Inhabited ⟪ A × B → B ⟫ := ⟨
+  .lam ⟪A × B⟫ <| .snd <| .var 0,
+  lam <| snd <| var rfl
+⟩
+
+theorem AND₃ : Inhabited ⟪ A → B → A × B ⟫ := ⟨
+  .lam A <| .lam B <| .pair (.var 1) (.var 0),
+  by 
+    apply lam <| lam <| pair _ _
+    <;> apply var (by rfl)
+⟩
+
+theorem OR₁ : Inhabited ⟪ A → A + B ⟫ := ⟨
+  .lam A <| .inl (.var 0),
+  lam <| inl <| var rfl
+⟩
+
+theorem OR₂ : Inhabited ⟪ B → A + B ⟫ := ⟨
+  .lam B <| .inr (.var 0),
+  lam <| inr <| var rfl
+⟩
+
+theorem OR₃ : Inhabited ⟪ (A → C) → (B → C) → A + B → C ⟫ := ⟨
+  .lam ⟪A → C⟫ <| .lam ⟪B → C⟫ <| .lam ⟪A+B⟫ <| .case (.var 0) 
+    (.app (.var 3) (.var 0))
+    (.app (.var 2) (.var 0)),
+  lam <| lam <| lam <| case (var rfl) (app _ (var rfl) (var rfl)) (app _ (var rfl) (var rfl))
+⟩
+
+theorem K : Inhabited ⟪ □(A → B) → □A → □B ⟫ := by
   refine ⟨
     .lam _ <| .lam _ <| .shut <| .app (.open <| .var 1) (.open <| .var 0),
     .lam <| .lam <| .shut ?h
   ⟩
-  rw [←List.nil_append 
+  rw [Context.addLock, ←List.nil_append 
       ([] :: Context.add (mod Modality.Box A) (Context.add (mod Modality.Box (.fun A B)) []))]
   apply WellTyped.app A <;> {
     apply WellTyped.open
     apply WellTyped.var
     rfl
   }
+
+end Completeness
+
+/-- If a term is welltyped under an empty context, then it is closed -/
+theorem closed_of_wellTyped_empty : (⊢ t : A) → t.IsClosed := by
+  simp only [Term.IsClosed]
+  suffices ∀ Γ,
+    (Γ ⊢ t : A) → (Term.IsClosedUpTo Γ.vars t)
+  from this []
+  intro Γ h
+  induction h
+  <;> simp_all [Term.IsClosedUpTo, Context.addLock]
+  next h => 
+    rcases List.get?_eq_some.mp h with ⟨h_lt, _⟩
+    apply Nat.lt_add_right _ _ _ h_lt
+  next ih =>
+    rw [Nat.add_comm, Nat.add_comm (List.length _), Nat.add_assoc]
+    apply Term.isClosedUpTo_add ih
+
+
+/-- Rule of necessitation -/
+theorem weaken_addLock_of_closed {t : Term} : (⊢ t : A) → ([[]] ⊢ t : A) := by
+  intro h_wt
+  have h_closed : t.IsClosedUpTo ([] : Context).length := closed_of_wellTyped_empty h_wt
+  generalize [] = Γ at h_wt h_closed ⊢
+  induction h_wt 
+  case var => 
+    contradiction
+  case lam ih =>
+    simp
+
+
+-- theorem weakenOne : (Γ ⊢ t : A) → (Γ' :: Γ) ⊢ t : A := by
+--   sorry
+
+-- theorem weaken (Γ' : Context) : (Γ ⊢ t : A) → (Γ' ++ Γ) ⊢ t : A := by
+--   intro h
+--   induction Γ'
+--   next => exact h
+--   next Γ'₀  Γ' ih =>
+--     have := weakenOne Γ'₀ ih
+
+/-- Show that every theorem of the axiomatic proof system is inhabited -/
+theorem complete : K.Proof A → (∃ t, ⊢ t : A) := by
+  suffices ∀ {n} (A : TypeScheme n) (f : Fin n → Ty),
+    K.Proof A → (∃t, ⊢ t : (A.substitute f)  )
+  by
+    intro h
+    specialize this A Fin.elim0 h
+    simp at this
+    exact this
+  intro n A f h
+  induction h
+  case «axiom» h =>
+    rcases h with ⟨⟨⟩|⟨⟩|⟨⟩|⟨⟩|⟨⟩|⟨⟩|⟨⟩|⟨⟩|⟨⟩|⟨⟩, h⟩ 
+    <;> simp[List.get?] at h
+    <;> (try rcases h with ⟨⟨⟩, ⟨⟩⟩)
+    . apply Completeness.THEN₁
+    . apply Completeness.THEN₂
+    . apply Completeness.AND₁
+    . apply Completeness.AND₂
+    . apply Completeness.AND₃
+    . apply Completeness.OR₁
+    . apply Completeness.OR₂
+    . apply Completeness.OR₃
+    . apply Completeness.K
+  case substitution g h_eq ih => 
+    specialize ih (fun i => (g i).substitute f)
+    rw [←TypeScheme.substitute_substitute, h_eq] at ih
+    apply ih
+  case necessitation ih => 
+    simp [substitute]
+    rcases ih f with ⟨t, ih⟩
+    use .shut t
+    apply shut
+  case modusPonens =>
+    sorry
+
+
+/-
+  # Soundness
+-/
+-- theorem sound : (∃ t, Γ ⊢ t : A) → K.Proof ⟦ Γ ⊢ _ : A ⟧ := by
+--   rintro ⟨t, h⟩
+--   induction h
+--   next Γ Γs v hv =>
+--     cases Γ
+--     next => contradiction
+--     next Γ_hd Γ_tl =>
+--       simp only [Context.denote]
+--       induction v
+--       next =>
+--         simp at hv
+--         subst hv
+--         apply THEN₁.substitution (fun
+--             | (0 : Fin 2) => Γ_hd
+--             | (1 : Fin 2) => ⟦ Γ_tl :: Γs ⊢ _ : Γ_hd ⟧
+--           )
+--         rfl
+--       next =>
+--         sorry
+--   next =>
+--     sorry
+--   next =>
+--     sorry
+--   next =>
+--     sorry
+--   next =>
+--     sorry
+--   next =>
+--     sorry
+--   next =>
+--     sorry
+--   next =>
+--     sorry
+--   next =>
+--     sorry
+--   next =>
+--     sorry
+
+end WellTyped
